end2end: no admits in [FetchOk.v]

processor/src/processor/FetchOk.v
@@ -65,92 +65,98 @@ Section FetchOk.
     #kpc = #rpc.
 
   Definition AddrAligned (addr: kword width) :=
-    split1 2 _ addr = WO~0~0.
+    split1 2 (nwidth - 2) addr = WO~0~0.
 
-  Definition mem_related (kmem: kword width -> kword width)
-             (rmem: mem): Prop :=
-    forall addr val,
-      AddrAligned addr ->
-      Memory.load_bytes 4 rmem addr = Some val /\
-      combine 4 val = wordToZ (kmem addr).
+  Definition makeAlignedXAddr (base: kword (width - 2)) (n: nat): word :=
+    Word.combine WO~0~0 (base ^+ natToWord (nwidth - 2)%nat n).
+
+  Fixpoint makeAlignedXAddrs (base: kword (width - 2)) (n: nat): XAddrs :=
+    match n with
+    | O => nil
+    | S n' => makeAlignedXAddr base n :: makeAlignedXAddrs base n'
+    end.
+
+  Lemma makeAlignedXAddrs_AddrAligned:
+    forall base n x,
+      In x (makeAlignedXAddrs base n) ->
+      AddrAligned x.
+  Proof.
+    induction n; intros; [exfalso; auto|].
+    destruct H.
+    - subst; reflexivity.
+    - auto.
+  Qed.
 
   (* set of executable addresses in the kami processor *)
   Definition kamiXAddrs: XAddrs :=
-    addXAddrRange (wzero _) instrMemSize nil.
+    (* addXAddrRange (wzero _) instrMemSize nil. *)
+    makeAlignedXAddrs (wzero _) instrMemSize.
 
-  Lemma kamiXAddrs_In_prop:
-    forall addr,
-      In addr kamiXAddrs ->
-      exists saddr: Word.word ninstrMemSizeLg,
-        addr =
-        eq_rect (2 + ninstrMemSizeLg + (32 - (2 + ninstrMemSizeLg)))%nat
-                Word.word
-                (Word.combine (Word.combine WO~0~0 saddr) (ZToWord _ 0))
-                nwidth
-                (eq_sym (width_inst_valid HinstrMemBound)).
+  Corollary kamiXAddrs_In_AddrAligned:
+    forall addr, In addr kamiXAddrs -> AddrAligned addr.
   Proof.
-    unfold kamiXAddrs; intros.
-    assert (exists saddr: Word.word ninstrMemSizeLg,
-               wzero (BinInt.Z.to_nat width) =
-               eq_rect (2 + ninstrMemSizeLg + (32 - (2 + ninstrMemSizeLg)))%nat
-                       Word.word
-                       (Word.combine (Word.combine WO~0~0 saddr) (ZToWord _ 0))
-                       nwidth
-                       (eq_sym (width_inst_valid HinstrMemBound))).
-    { exists (wzero _).
-      apply wordToZ_inj.
-      rewrite wordToZ_eq_rect.
-      rewrite ZToWord_zero.
-      rewrite combine_wzero.
-      rewrite (width_inst_valid HinstrMemBound).
-      reflexivity.
-    }
-
-    generalize dependent (wzero (BinInt.Z.to_nat width)).
-    induction instrMemSize; intros; [exfalso; auto|].
-    destruct H; [subst; assumption|].
-    eapply IHn; [eassumption|].
-    destruct H0 as [saddr ?]; subst.
-
-    exists (saddr ^+ $1).
-    change (word.of_Z 4) with (ZToWord nwidth 4).
-    replace (ZToWord nwidth 4)
-      with (eq_rect
-              (2 + ninstrMemSizeLg + (32 - (2 + ninstrMemSizeLg)))%nat
-              Word.word (ZToWord _ 4) nwidth
-              (eq_sym (width_inst_valid HinstrMemBound))).
-    2: {
-      apply wordToZ_inj.
-      rewrite wordToZ_eq_rect.
-      rewrite (width_inst_valid HinstrMemBound).
-      reflexivity.
-    }
-    cbv [word.add word WordsKami wordW KamiWord.word].
-    rewrite <-eq_rect_wplus.
-
-    f_equal.
-    case TODO_joonwon.
-
+    intros.
+    eapply makeAlignedXAddrs_AddrAligned; eassumption.
   Qed.
+
+  Lemma pc_related_preserves_AddrAligned:
+    forall kpc rpc,
+      pc_related kpc rpc -> AddrAligned rpc ->
+      split1 2 _ kpc = WO~0~0.
+  Proof.
+    unfold pc_related, AddrAligned; intros.
+
+    pose proof (Word.combine_split 2 ninstrMemSizeLg kpc).
+    rewrite <-H1 in H.
+    remember (split1 2 ninstrMemSizeLg kpc) as kpcl; clear Heqkpcl.
+    remember (split2 2 ninstrMemSizeLg kpc) as kpcr; clear Heqkpcr.
+    clear H1 kpc.
+
+    pose proof (Word.combine_split 2 (nwidth - 2) rpc).
+    rewrite <-H1 in H.
+    remember (split1 2 (nwidth - 2) rpc) as rpcl; clear Heqrpcl.
+    remember (split2 2 (nwidth - 2) rpc) as rpcr; clear Heqrpcr.
+    clear H1 rpc; subst rpcl.
+
+    rewrite wordToNat_combine in H.
+    change (Z.to_nat width) with (2 + (nwidth - 2))%nat in H.
+    rewrite wordToNat_combine in H.
+
+    change (NatLib.pow2 2) with 4%nat in H.
+    do 2 rewrite Nat.mul_comm with (n:= 4%nat) in H.
+    apply f_equal with (f:= fun x => Nat.modulo x 4%nat) in H.
+    do 2 rewrite Nat.mod_add in H by discriminate.
+    do 2 rewrite Nat.mod_small in H by apply wordToNat_bound.
+    apply wordToNat_inj; assumption.
+  Qed.
+
+  Definition mem_related (kmem: kword width -> kword width)
+             (rmem: mem): Prop :=
+    forall addr,
+      AddrAligned addr ->
+      exists val,
+        Memory.load_bytes 4 rmem addr = Some val /\
+        combine 4 val = wordToZ (kmem addr).
 
   Definition RiscvXAddrsSafe
              (kmemi: kword instrMemSizeLg -> kword width)
              (kmemd: kword width -> kword width)
              (xaddrs: XAddrs) :=
-    forall kpc rpc,
+    forall rpc,
       isXAddr rpc xaddrs ->
-      pc_related kpc rpc ->
-      kmemd rpc = kmemi (split2 2 _ kpc).
+      AddrAligned rpc /\
+      (forall kpc, pc_related kpc rpc ->
+                   kmemd rpc = kmemi (split2 2 _ kpc)).
 
   Lemma rv32AlignAddr_consistent:
     forall rpc kpc,
       In rpc kamiXAddrs ->
       pc_related kpc rpc ->
-      rpc = evalExpr
-              (IsaRv32.rv32AlignAddr
-                 32%nat (Z.to_nat instrMemSizeLg)
-                 (width_inst_valid HinstrMemBound)
-                 type (split2 2 (Z.to_nat instrMemSizeLg) kpc)).
+      evalExpr
+        (IsaRv32.rv32AlignAddr
+           32%nat (Z.to_nat instrMemSizeLg)
+           (width_inst_valid HinstrMemBound)
+           type (split2 2 (Z.to_nat instrMemSizeLg) kpc)) = rpc.
   Proof.
     intros.
     cbv [IsaRv32.rv32AlignAddr].
@@ -158,15 +164,21 @@ Section FetchOk.
     cbv [evalExpr evalBinBit evalUniBit].
     cbv [evalConstT].
 
-    apply kamiXAddrs_In_prop in H.
-    destruct H as [saddr ?].
-    rewrite H at 1.
-    repeat f_equal.
+    apply wordToNat_inj.
+    rewrite wordToNat_eq_rect.
+    do 2 rewrite wordToNat_combine.
+    do 2 rewrite ZToWord_zero.
+    do 2 rewrite wordToNat_wzero.
+    rewrite Nat.mul_0_r, Nat.add_0_r, Nat.add_0_l.
 
-    subst.
-    red in H0.
-    rewrite wordToNat_eq_rect in H0.
-    case TODO_joonwon.
+    rewrite <-H0.
+    rewrite <-(Word.combine_split 2 ninstrMemSizeLg kpc) at 2.
+
+    apply kamiXAddrs_In_AddrAligned in H.
+    pose proof (pc_related_preserves_AddrAligned _ _ H0 H).
+    rewrite H1.
+    rewrite wordToNat_combine.
+    reflexivity.
   Qed.
 
   Lemma fetch_ok:
@@ -184,7 +196,14 @@ Section FetchOk.
         Memory.load_bytes 4 rmemd rpc = Some rinst /\
         combine 4 rinst = wordToZ (kmemi (split2 2 _ kpc)).
   Proof.
-    case TODO_joonwon.
+    intros.
+    specialize (Hxs _ H); destruct Hxs.
+    specialize (H3 _ H0).
+    specialize (H1 _ H2).
+    destruct H1 as (rinst & ? & ?).
+    exists rinst.
+    split; [assumption|].
+    congruence.
   Qed.
 
 End FetchOk.
